- add bot_like to ott

proof/old_system/uni/def_ott.v
@@ -40,16 +40,16 @@ with contd : Set :=
  | contd_infapp (e:exp) (cs:conts)
  | contd_unioninfabs (A:typ) (B:typ) (cd:contd).
 
-Inductive dbind : Set := 
- | dbind_tvar_empty : dbind
- | dbind_stvar_empty : dbind
- | dbind_typ (A:typ).
-
 Inductive abind : Set := 
  | abind_tvar_empty : abind
  | abind_stvar_empty : abind
  | abind_etvar_empty : abind
  | abind_var_typ (A:typ).
+
+Inductive dbind : Set := 
+ | dbind_tvar_empty : dbind
+ | dbind_stvar_empty : dbind
+ | dbind_typ (A:typ).
 
 Inductive work : Set := 
  | work_infer (e:exp) (cs:conts)
@@ -65,9 +65,9 @@ Inductive work : Set :=
  | work_applys (cs:conts) (A:typ)
  | work_applyd (cd:contd) (A:typ) (B:typ).
 
-Definition denv : Set := list (atom*dbind).
-
 Definition aenv : Set := list (atom*abind).
+
+Definition denv : Set := list (atom*dbind).
 
 Inductive aworklist : Set := 
  | aworklist_empty : aworklist
@@ -103,22 +103,6 @@ Fixpoint open_typ_wrt_typ_rec (k:nat) (A_5:typ) (A__6:typ) {struct A__6}: typ :=
   | (typ_intersection A1 A2) => typ_intersection (open_typ_wrt_typ_rec k A_5 A1) (open_typ_wrt_typ_rec k A_5 A2)
 end.
 
-Fixpoint open_exp_wrt_typ_rec (k:nat) (A_5:typ) (e_5:exp) {struct e_5}: exp :=
-  match e_5 with
-  | exp_unit => exp_unit 
-  | (exp_var_b nat) => exp_var_b nat
-  | (exp_var_f x) => exp_var_f x
-  | (exp_abs e) => exp_abs (open_exp_wrt_typ_rec k A_5 e)
-  | (exp_app e1 e2) => exp_app (open_exp_wrt_typ_rec k A_5 e1) (open_exp_wrt_typ_rec k A_5 e2)
-  | (exp_tabs body5) => exp_tabs (open_body_wrt_typ_rec (S k) A_5 body5)
-  | (exp_tapp e A) => exp_tapp (open_exp_wrt_typ_rec k A_5 e) (open_typ_wrt_typ_rec k A_5 A)
-  | (exp_anno e A) => exp_anno (open_exp_wrt_typ_rec k A_5 e) (open_typ_wrt_typ_rec k A_5 A)
-end
-with open_body_wrt_typ_rec (k:nat) (A5:typ) (body5:body) : body :=
-  match body5 with
-  | (body_anno e A) => body_anno (open_exp_wrt_typ_rec k A5 e) (open_typ_wrt_typ_rec k A5 A)
-end.
-
 Fixpoint open_exp_wrt_exp_rec (k:nat) (e_5:exp) (e__6:exp) {struct e__6}: exp :=
   match e__6 with
   | exp_unit => exp_unit 
@@ -140,19 +124,20 @@ with open_body_wrt_exp_rec (k:nat) (e5:exp) (body5:body) : body :=
   | (body_anno e A) => body_anno (open_exp_wrt_exp_rec k e5 e) A
 end.
 
-Fixpoint open_contd_wrt_typ_rec (k:nat) (A5:typ) (cd5:contd) {struct cd5}: contd :=
-  match cd5 with
-  | (contd_infabsunion A cd) => contd_infabsunion (open_typ_wrt_typ_rec k A5 A) (open_contd_wrt_typ_rec k A5 cd)
-  | (contd_infapp e cs) => contd_infapp (open_exp_wrt_typ_rec k A5 e) (open_conts_wrt_typ_rec k A5 cs)
-  | (contd_unioninfabs A B cd) => contd_unioninfabs (open_typ_wrt_typ_rec k A5 A) (open_typ_wrt_typ_rec k A5 B) (open_contd_wrt_typ_rec k A5 cd)
+Fixpoint open_exp_wrt_typ_rec (k:nat) (A_5:typ) (e_5:exp) {struct e_5}: exp :=
+  match e_5 with
+  | exp_unit => exp_unit 
+  | (exp_var_b nat) => exp_var_b nat
+  | (exp_var_f x) => exp_var_f x
+  | (exp_abs e) => exp_abs (open_exp_wrt_typ_rec k A_5 e)
+  | (exp_app e1 e2) => exp_app (open_exp_wrt_typ_rec k A_5 e1) (open_exp_wrt_typ_rec k A_5 e2)
+  | (exp_tabs body5) => exp_tabs (open_body_wrt_typ_rec (S k) A_5 body5)
+  | (exp_tapp e A) => exp_tapp (open_exp_wrt_typ_rec k A_5 e) (open_typ_wrt_typ_rec k A_5 A)
+  | (exp_anno e A) => exp_anno (open_exp_wrt_typ_rec k A_5 e) (open_typ_wrt_typ_rec k A_5 A)
 end
-with open_conts_wrt_typ_rec (k:nat) (A_5:typ) (cs5:conts) {struct cs5}: conts :=
-  match cs5 with
-  | (conts_infabs cd) => conts_infabs (open_contd_wrt_typ_rec k A_5 cd)
-  | (conts_inftapp A cs) => conts_inftapp (open_typ_wrt_typ_rec k A_5 A) (open_conts_wrt_typ_rec k A_5 cs)
-  | (conts_inftappunion A1 A2 cs) => conts_inftappunion (open_typ_wrt_typ_rec k A_5 A1) (open_typ_wrt_typ_rec k A_5 A2) (open_conts_wrt_typ_rec k A_5 cs)
-  | (conts_unioninftapp A2 cs) => conts_unioninftapp (open_typ_wrt_typ_rec k A_5 A2) (open_conts_wrt_typ_rec k A_5 cs)
-  | (conts_sub A) => conts_sub (open_typ_wrt_typ_rec k A_5 A)
+with open_body_wrt_typ_rec (k:nat) (A5:typ) (body5:body) : body :=
+  match body5 with
+  | (body_anno e A) => body_anno (open_exp_wrt_typ_rec k A5 e) (open_typ_wrt_typ_rec k A5 A)
 end.
 
 Fixpoint open_contd_wrt_exp_rec (k:nat) (e5:exp) (cd5:contd) {struct cd5}: contd :=
@@ -170,28 +155,19 @@ with open_conts_wrt_exp_rec (k:nat) (e5:exp) (cs5:conts) {struct cs5}: conts :=
   | (conts_sub A) => conts_sub A
 end.
 
-Definition open_work_wrt_typ_rec (k:nat) (A_5:typ) (w5:work) : work :=
-  match w5 with
-  | (work_infer e cs) => work_infer (open_exp_wrt_typ_rec k A_5 e) (open_conts_wrt_typ_rec k A_5 cs)
-  | (work_check e A) => work_check (open_exp_wrt_typ_rec k A_5 e) (open_typ_wrt_typ_rec k A_5 A)
-  | (work_infabs A cd) => work_infabs (open_typ_wrt_typ_rec k A_5 A) (open_contd_wrt_typ_rec k A_5 cd)
-  | (work_infabsunion A1 B1 A2 cd) => work_infabsunion (open_typ_wrt_typ_rec k A_5 A1) (open_typ_wrt_typ_rec k A_5 B1) (open_typ_wrt_typ_rec k A_5 A2) (open_contd_wrt_typ_rec k A_5 cd)
-  | (work_infapp A B e cs) => work_infapp (open_typ_wrt_typ_rec k A_5 A) (open_typ_wrt_typ_rec k A_5 B) (open_exp_wrt_typ_rec k A_5 e) (open_conts_wrt_typ_rec k A_5 cs)
-  | (work_inftapp A1 A2 cs) => work_inftapp (open_typ_wrt_typ_rec k A_5 A1) (open_typ_wrt_typ_rec k A_5 A2) (open_conts_wrt_typ_rec k A_5 cs)
-  | (work_sub A1 A2) => work_sub (open_typ_wrt_typ_rec k A_5 A1) (open_typ_wrt_typ_rec k A_5 A2)
-  | (work_inftappunion A1 A2 B cs) => work_inftappunion (open_typ_wrt_typ_rec k A_5 A1) (open_typ_wrt_typ_rec k A_5 A2) (open_typ_wrt_typ_rec k A_5 B) (open_conts_wrt_typ_rec k A_5 cs)
-  | (work_unioninftapp A1 A2 cs) => work_unioninftapp (open_typ_wrt_typ_rec k A_5 A1) (open_typ_wrt_typ_rec k A_5 A2) (open_conts_wrt_typ_rec k A_5 cs)
-  | (work_unioninfabs A1 B1 A2 B2 cd) => work_unioninfabs (open_typ_wrt_typ_rec k A_5 A1) (open_typ_wrt_typ_rec k A_5 B1) (open_typ_wrt_typ_rec k A_5 A2) (open_typ_wrt_typ_rec k A_5 B2) (open_contd_wrt_typ_rec k A_5 cd)
-  | (work_applys cs A) => work_applys (open_conts_wrt_typ_rec k A_5 cs) (open_typ_wrt_typ_rec k A_5 A)
-  | (work_applyd cd A B) => work_applyd (open_contd_wrt_typ_rec k A_5 cd) (open_typ_wrt_typ_rec k A_5 A) (open_typ_wrt_typ_rec k A_5 B)
-end.
-
-Definition open_abind_wrt_typ_rec (k:nat) (A5:typ) (ab5:abind) : abind :=
-  match ab5 with
-  | abind_tvar_empty => abind_tvar_empty 
-  | abind_stvar_empty => abind_stvar_empty 
-  | abind_etvar_empty => abind_etvar_empty 
-  | (abind_var_typ A) => abind_var_typ (open_typ_wrt_typ_rec k A5 A)
+Fixpoint open_contd_wrt_typ_rec (k:nat) (A5:typ) (cd5:contd) {struct cd5}: contd :=
+  match cd5 with
+  | (contd_infabsunion A cd) => contd_infabsunion (open_typ_wrt_typ_rec k A5 A) (open_contd_wrt_typ_rec k A5 cd)
+  | (contd_infapp e cs) => contd_infapp (open_exp_wrt_typ_rec k A5 e) (open_conts_wrt_typ_rec k A5 cs)
+  | (contd_unioninfabs A B cd) => contd_unioninfabs (open_typ_wrt_typ_rec k A5 A) (open_typ_wrt_typ_rec k A5 B) (open_contd_wrt_typ_rec k A5 cd)
+end
+with open_conts_wrt_typ_rec (k:nat) (A_5:typ) (cs5:conts) {struct cs5}: conts :=
+  match cs5 with
+  | (conts_infabs cd) => conts_infabs (open_contd_wrt_typ_rec k A_5 cd)
+  | (conts_inftapp A cs) => conts_inftapp (open_typ_wrt_typ_rec k A_5 A) (open_conts_wrt_typ_rec k A_5 cs)
+  | (conts_inftappunion A1 A2 cs) => conts_inftappunion (open_typ_wrt_typ_rec k A_5 A1) (open_typ_wrt_typ_rec k A_5 A2) (open_conts_wrt_typ_rec k A_5 cs)
+  | (conts_unioninftapp A2 cs) => conts_unioninftapp (open_typ_wrt_typ_rec k A_5 A2) (open_conts_wrt_typ_rec k A_5 cs)
+  | (conts_sub A) => conts_sub (open_typ_wrt_typ_rec k A_5 A)
 end.
 
 Definition open_work_wrt_exp_rec (k:nat) (e5:exp) (w5:work) : work :=
@@ -210,18 +186,35 @@ Definition open_work_wrt_exp_rec (k:nat) (e5:exp) (w5:work) : work :=
   | (work_applyd cd A B) => work_applyd (open_contd_wrt_exp_rec k e5 cd) A B
 end.
 
+Definition open_abind_wrt_typ_rec (k:nat) (A5:typ) (ab5:abind) : abind :=
+  match ab5 with
+  | abind_tvar_empty => abind_tvar_empty 
+  | abind_stvar_empty => abind_stvar_empty 
+  | abind_etvar_empty => abind_etvar_empty 
+  | (abind_var_typ A) => abind_var_typ (open_typ_wrt_typ_rec k A5 A)
+end.
+
+Definition open_work_wrt_typ_rec (k:nat) (A_5:typ) (w5:work) : work :=
+  match w5 with
+  | (work_infer e cs) => work_infer (open_exp_wrt_typ_rec k A_5 e) (open_conts_wrt_typ_rec k A_5 cs)
+  | (work_check e A) => work_check (open_exp_wrt_typ_rec k A_5 e) (open_typ_wrt_typ_rec k A_5 A)
+  | (work_infabs A cd) => work_infabs (open_typ_wrt_typ_rec k A_5 A) (open_contd_wrt_typ_rec k A_5 cd)
+  | (work_infabsunion A1 B1 A2 cd) => work_infabsunion (open_typ_wrt_typ_rec k A_5 A1) (open_typ_wrt_typ_rec k A_5 B1) (open_typ_wrt_typ_rec k A_5 A2) (open_contd_wrt_typ_rec k A_5 cd)
+  | (work_infapp A B e cs) => work_infapp (open_typ_wrt_typ_rec k A_5 A) (open_typ_wrt_typ_rec k A_5 B) (open_exp_wrt_typ_rec k A_5 e) (open_conts_wrt_typ_rec k A_5 cs)
+  | (work_inftapp A1 A2 cs) => work_inftapp (open_typ_wrt_typ_rec k A_5 A1) (open_typ_wrt_typ_rec k A_5 A2) (open_conts_wrt_typ_rec k A_5 cs)
+  | (work_sub A1 A2) => work_sub (open_typ_wrt_typ_rec k A_5 A1) (open_typ_wrt_typ_rec k A_5 A2)
+  | (work_inftappunion A1 A2 B cs) => work_inftappunion (open_typ_wrt_typ_rec k A_5 A1) (open_typ_wrt_typ_rec k A_5 A2) (open_typ_wrt_typ_rec k A_5 B) (open_conts_wrt_typ_rec k A_5 cs)
+  | (work_unioninftapp A1 A2 cs) => work_unioninftapp (open_typ_wrt_typ_rec k A_5 A1) (open_typ_wrt_typ_rec k A_5 A2) (open_conts_wrt_typ_rec k A_5 cs)
+  | (work_unioninfabs A1 B1 A2 B2 cd) => work_unioninfabs (open_typ_wrt_typ_rec k A_5 A1) (open_typ_wrt_typ_rec k A_5 B1) (open_typ_wrt_typ_rec k A_5 A2) (open_typ_wrt_typ_rec k A_5 B2) (open_contd_wrt_typ_rec k A_5 cd)
+  | (work_applys cs A) => work_applys (open_conts_wrt_typ_rec k A_5 cs) (open_typ_wrt_typ_rec k A_5 A)
+  | (work_applyd cd A B) => work_applyd (open_contd_wrt_typ_rec k A_5 cd) (open_typ_wrt_typ_rec k A_5 A) (open_typ_wrt_typ_rec k A_5 B)
+end.
+
 Definition open_dbind_wrt_typ_rec (k:nat) (A5:typ) (db5:dbind) : dbind :=
   match db5 with
   | dbind_tvar_empty => dbind_tvar_empty 
   | dbind_stvar_empty => dbind_stvar_empty 
   | (dbind_typ A) => dbind_typ (open_typ_wrt_typ_rec k A5 A)
-end.
-
-Fixpoint open_aworklist_wrt_typ_rec (k:nat) (A5:typ) (Γ_5:aworklist) {struct Γ_5}: aworklist :=
-  match Γ_5 with
-  | aworklist_empty => aworklist_empty 
-  | (aworklist_cons_var Γ X ab) => aworklist_cons_var (open_aworklist_wrt_typ_rec k A5 Γ) X (open_abind_wrt_typ_rec k A5 ab)
-  | (aworklist_cons_work Γ w) => aworklist_cons_work (open_aworklist_wrt_typ_rec k A5 Γ) (open_work_wrt_typ_rec k A5 w)
 end.
 
 Fixpoint open_aworklist_wrt_exp_rec (k:nat) (e5:exp) (Γ_5:aworklist) {struct Γ_5}: aworklist :=
@@ -231,11 +224,11 @@ Fixpoint open_aworklist_wrt_exp_rec (k:nat) (e5:exp) (Γ_5:aworklist) {struct Γ
   | (aworklist_cons_work Γ w) => aworklist_cons_work (open_aworklist_wrt_exp_rec k e5 Γ) (open_work_wrt_exp_rec k e5 w)
 end.
 
-Fixpoint open_dworklist_wrt_exp_rec (k:nat) (e5:exp) (Ω5:dworklist) {struct Ω5}: dworklist :=
-  match Ω5 with
-  | dworklist_empty => dworklist_empty 
-  | (dworklist_cons_var Ω X db) => dworklist_cons_var (open_dworklist_wrt_exp_rec k e5 Ω) X db
-  | (dworklist_cons_work Ω w) => dworklist_cons_work (open_dworklist_wrt_exp_rec k e5 Ω) (open_work_wrt_exp_rec k e5 w)
+Fixpoint open_aworklist_wrt_typ_rec (k:nat) (A5:typ) (Γ_5:aworklist) {struct Γ_5}: aworklist :=
+  match Γ_5 with
+  | aworklist_empty => aworklist_empty 
+  | (aworklist_cons_var Γ X ab) => aworklist_cons_var (open_aworklist_wrt_typ_rec k A5 Γ) X (open_abind_wrt_typ_rec k A5 ab)
+  | (aworklist_cons_work Γ w) => aworklist_cons_work (open_aworklist_wrt_typ_rec k A5 Γ) (open_work_wrt_typ_rec k A5 w)
 end.
 
 Fixpoint open_dworklist_wrt_typ_rec (k:nat) (A5:typ) (Ω5:dworklist) {struct Ω5}: dworklist :=
@@ -245,39 +238,46 @@ Fixpoint open_dworklist_wrt_typ_rec (k:nat) (A5:typ) (Ω5:dworklist) {struct Ω5
   | (dworklist_cons_work Ω w) => dworklist_cons_work (open_dworklist_wrt_typ_rec k A5 Ω) (open_work_wrt_typ_rec k A5 w)
 end.
 
-Definition open_aworklist_wrt_typ A5 Γ_5 := open_aworklist_wrt_typ_rec 0 Γ_5 A5.
-
-Definition open_abind_wrt_typ A5 ab5 := open_abind_wrt_typ_rec 0 ab5 A5.
-
-Definition open_contd_wrt_typ A5 cd5 := open_contd_wrt_typ_rec 0 cd5 A5.
-
-Definition open_work_wrt_typ A_5 w5 := open_work_wrt_typ_rec 0 w5 A_5.
-
-Definition open_dbind_wrt_typ A5 db5 := open_dbind_wrt_typ_rec 0 db5 A5.
+Fixpoint open_dworklist_wrt_exp_rec (k:nat) (e5:exp) (Ω5:dworklist) {struct Ω5}: dworklist :=
+  match Ω5 with
+  | dworklist_empty => dworklist_empty 
+  | (dworklist_cons_var Ω X db) => dworklist_cons_var (open_dworklist_wrt_exp_rec k e5 Ω) X db
+  | (dworklist_cons_work Ω w) => dworklist_cons_work (open_dworklist_wrt_exp_rec k e5 Ω) (open_work_wrt_exp_rec k e5 w)
+end.
 
 Definition open_aworklist_wrt_exp e5 Γ_5 := open_aworklist_wrt_exp_rec 0 Γ_5 e5.
 
 Definition open_exp_wrt_exp e_5 e__6 := open_exp_wrt_exp_rec 0 e__6 e_5.
 
-Definition open_conts_wrt_exp e5 cs5 := open_conts_wrt_exp_rec 0 cs5 e5.
+Definition open_body_wrt_exp e5 body5 := open_body_wrt_exp_rec 0 body5 e5.
 
-Definition open_dworklist_wrt_exp e5 Ω5 := open_dworklist_wrt_exp_rec 0 Ω5 e5.
+Definition open_aworklist_wrt_typ A5 Γ_5 := open_aworklist_wrt_typ_rec 0 Γ_5 A5.
 
 Definition open_exp_wrt_typ A_5 e_5 := open_exp_wrt_typ_rec 0 e_5 A_5.
 
-Definition open_body_wrt_typ A5 body5 := open_body_wrt_typ_rec 0 body5 A5.
+Definition open_contd_wrt_exp e5 cd5 := open_contd_wrt_exp_rec 0 cd5 e5.
+
+Definition open_work_wrt_typ A_5 w5 := open_work_wrt_typ_rec 0 w5 A_5.
 
 Definition open_conts_wrt_typ A_5 cs5 := open_conts_wrt_typ_rec 0 cs5 A_5.
 
-Definition open_typ_wrt_typ A_5 A__6 := open_typ_wrt_typ_rec 0 A__6 A_5.
+Definition open_dbind_wrt_typ A5 db5 := open_dbind_wrt_typ_rec 0 db5 A5.
 
-Definition open_contd_wrt_exp e5 cd5 := open_contd_wrt_exp_rec 0 cd5 e5.
+Definition open_abind_wrt_typ A5 ab5 := open_abind_wrt_typ_rec 0 ab5 A5.
 
 Definition open_work_wrt_exp e5 w5 := open_work_wrt_exp_rec 0 w5 e5.
 
+Definition open_contd_wrt_typ A5 cd5 := open_contd_wrt_typ_rec 0 cd5 A5.
+
+Definition open_body_wrt_typ A5 body5 := open_body_wrt_typ_rec 0 body5 A5.
+
 Definition open_dworklist_wrt_typ A5 Ω5 := open_dworklist_wrt_typ_rec 0 Ω5 A5.
 
-Definition open_body_wrt_exp e5 body5 := open_body_wrt_exp_rec 0 body5 e5.
+Definition open_typ_wrt_typ A_5 A__6 := open_typ_wrt_typ_rec 0 A__6 A_5.
+
+Definition open_conts_wrt_exp e5 cs5 := open_conts_wrt_exp_rec 0 cs5 e5.
+
+Definition open_dworklist_wrt_exp e5 Ω5 := open_dworklist_wrt_exp_rec 0 Ω5 e5.
 
 (** closing up abstractions *)
 Fixpoint close_typ_wrt_typ_rec (k:nat) (A_5:var) (A__6:typ) {struct A__6}: typ :=
@@ -565,16 +565,6 @@ with lc_conts : conts -> Prop :=    (* defn lc_conts *)
      (lc_typ A) ->
      (lc_conts (conts_sub A)).
 
-(* defns LC_dbind *)
-Inductive lc_dbind : dbind -> Prop :=    (* defn lc_dbind *)
- | lc_dbind_tvar_empty : 
-     (lc_dbind dbind_tvar_empty)
- | lc_dbind_stvar_empty : 
-     (lc_dbind dbind_stvar_empty)
- | lc_dbind_typ : forall (A:typ),
-     (lc_typ A) ->
-     (lc_dbind (dbind_typ A)).
-
 (* defns LC_abind *)
 Inductive lc_abind : abind -> Prop :=    (* defn lc_abind *)
  | lc_abind_tvar_empty : 
@@ -586,6 +576,16 @@ Inductive lc_abind : abind -> Prop :=    (* defn lc_abind *)
  | lc_abind_var_typ : forall (A:typ),
      (lc_typ A) ->
      (lc_abind (abind_var_typ A)).
+
+(* defns LC_dbind *)
+Inductive lc_dbind : dbind -> Prop :=    (* defn lc_dbind *)
+ | lc_dbind_tvar_empty : 
+     (lc_dbind dbind_tvar_empty)
+ | lc_dbind_stvar_empty : 
+     (lc_dbind dbind_stvar_empty)
+ | lc_dbind_typ : forall (A:typ),
+     (lc_typ A) ->
+     (lc_dbind (dbind_typ A)).
 
 (* defns LC_work *)
 Inductive lc_work : work -> Prop :=    (* defn lc_work *)
@@ -1334,6 +1334,26 @@ Inductive d_wf_work : denv -> work -> Prop :=    (* defn d_wf_work *)
      d_wf_contd Ψ cd ->
      d_wf_work Ψ (work_applyd cd A B).
 
+(* defns typ_bot_like *)
+Inductive typ_bot_like : typ -> Prop :=    (* defn typ_bot_like *)
+ | typ_bl__bot : 
+     typ_bot_like typ_bot
+ | typ_bl__intersection1 : forall (A B:typ),
+     lc_typ B ->
+     typ_bot_like A ->
+     typ_bot_like (typ_intersection A B)
+ | typ_bl__intersection2 : forall (A B:typ),
+     lc_typ A ->
+     typ_bot_like B ->
+     typ_bot_like (typ_intersection A B)
+ | typ_bl__intersection1 : forall (A B:typ),
+     typ_bot_like A ->
+     typ_bot_like B ->
+     typ_bot_like (typ_union A B)
+ | typ_bl__all : forall (L:vars) (A:typ),
+      ( forall X , X \notin  L  -> typ_bot_like  ( open_typ_wrt_typ A (typ_var_f X) )  )  ->
+     typ_bot_like (typ_all A).
+
 (* defns Jd_wf_twl *)
 Inductive d_wf_twl : dworklist -> Prop :=    (* defn d_wf_twl *)
  | d_wf_twl__empty : 
@@ -1417,15 +1437,14 @@ Inductive d_sub : denv -> typ -> typ -> Prop :=    (* defn d_sub *)
      d_sub Ψ A2 B2 ->
      d_sub Ψ (typ_arrow A1 A2) (typ_arrow B1 B2)
  | d_sub__all : forall (L:vars) (Ψ:denv) (A B:typ),
-      ( forall X , X \notin  L  -> d_sneq_stvar  ( X ~ dbind_tvar_empty  ++  Ψ )   ( open_typ_wrt_typ A (typ_var_f X) )  )  ->
-      ( forall X , X \notin  L  -> d_sneq_stvar  ( X ~ dbind_tvar_empty  ++  Ψ )   ( open_typ_wrt_typ B (typ_var_f X) )  )  ->
+      ( forall X , X \notin  L  ->  (  (  ( d_sneq_stvar  ( X ~ dbind_tvar_empty  ++  Ψ )   ( open_typ_wrt_typ A (typ_var_f X) )  ) /\ ( d_sneq_stvar  ( X ~ dbind_tvar_empty  ++  Ψ )   ( open_typ_wrt_typ B (typ_var_f X) )  )  )  ) \/ ( typ_bot_like (typ_all A) )  )  ->
       ( forall X , X \notin  L  -> d_sub  ( X ~ dbind_stvar_empty  ++  Ψ )   ( open_typ_wrt_typ A (typ_var_f X) )   ( open_typ_wrt_typ B (typ_var_f X) )  )  ->
      d_sub Ψ (typ_all A) (typ_all B)
  | d_sub__alll : forall (L:vars) (Ψ:denv) (A B T:typ),
      neq_all B ->
      neq_intersection B ->
      neq_union B ->
-      ( forall X , X \notin  L  -> d_sneq_stvar  ( X ~ dbind_tvar_empty  ++  Ψ )   ( open_typ_wrt_typ A (typ_var_f X) )  )  ->
+      ( forall X , X \notin  L  ->  ( d_sneq_stvar  ( X ~ dbind_tvar_empty  ++  Ψ )   ( open_typ_wrt_typ A (typ_var_f X) )  ) \/ ( typ_bot_like (typ_all A) )  )  ->
      d_mono_typ Ψ T ->
      d_sub Ψ  (open_typ_wrt_typ  A   T )  B ->
      d_sub Ψ (typ_all A) B
@@ -1725,6 +1744,6 @@ Inductive a_wf_env : aenv -> Prop :=    (* defn a_wf_env *)
 
 
 (** infrastructure *)
-#[export] Hint Constructors s_in s_in_b neq_abs neq_all neq_intersection neq_union neq_bot d_wf_typ d_wf_exp d_wf_body d_wf_tenv d_wf_env d_mono_typ d_wf_conts d_wf_contd d_wf_work d_wf_twl d_wf_wl d_sneq_stvar d_sub a_wf_typ a_mono_typ a_wf_exp a_wf_body a_wf_conts a_wf_contd a_wf_work a_wf_wwl a_wf_twl a_wf_wl a_wf_env lc_typ lc_exp lc_body lc_contd lc_conts lc_dbind lc_abind lc_work lc_aworklist lc_dworklist : core.
+#[export] Hint Constructors s_in s_in_b neq_abs neq_all neq_intersection neq_union neq_bot d_wf_typ d_wf_exp d_wf_body d_wf_tenv d_wf_env d_mono_typ d_wf_conts d_wf_contd d_wf_work typ_bot_like d_wf_twl d_wf_wl d_sneq_stvar d_sub a_wf_typ a_mono_typ a_wf_exp a_wf_body a_wf_conts a_wf_contd a_wf_work a_wf_wwl a_wf_twl a_wf_wl a_wf_env lc_typ lc_exp lc_body lc_contd lc_conts lc_abind lc_dbind lc_work lc_aworklist lc_dworklist : core.
 
 
